Fifo.v
@@ -3,40 +3,12 @@ Set Implicit Arguments.
 Require Import CpdtTactics.
 Require Import Arith.
 
-(* basic nat lemma *)
-Definition predLess (n m : nat) : n < m -> pred n < m.
-  crush.
-Qed.
-
-(* Fifo environment *)
 Section Fifo.
 Variable A : Set.
 
-(* size of Fifo *)
-Variable size : nat.
-
-(* enq is protected to not exceed size *)
 Inductive Fifo : nat -> Set :=
-| emptyFifo : Fifo 0
-| enq : A -> forall n, Fifo n -> n < size -> Fifo (S n).
-
-(*
-Definition unitA n := match n with
-                      | 0 => unit
-                      | S _ => A
-                      end.
-
-Fixpoint first' n (f : Fifo n) : unitA n :=
-  match f in Fifo n return unitA n with
-  | emptyFifo => tt
-  | enq x _ f _ => match f in Fifo n return (unitA n) -> A with
-                   | emptyFifo => fun _ => x
-                   | enq _ _ _ _ => fun first_f => first_f
-                   end (first' f)
-  end.
-
-Definition first n (f : Fifo (S n)) : A := first' f.
-*)
+| null : Fifo 0
+| store : A -> forall n, Fifo n -> Fifo (S n).
 
 Definition s_n_0 n (pf : S n = 0) : False :=
   match pf in (_ = e) return match e with
@@ -48,99 +20,65 @@ Definition s_n_0 n (pf : S n = 0) : False :=
 
 Fixpoint first' n (f : Fifo n) : forall m, S m = n -> A :=
   match f in Fifo n0 return forall m, S m = n0 -> A with
-  | emptyFifo => fun _ pf0 => match s_n_0 pf0 with end
-  | enq x _ f1 _ => fun _ _ => match f1 in (Fifo n2) return (forall m, S m = n2 -> A) -> A with
-                               | emptyFifo => fun _ => x
-                                 | enq _ n3 _ _ => fun val_pf => val_pf n3 eq_refl
+  | null => fun _ pf0 => match s_n_0 pf0 with end
+  | store x _ f1 => fun _ _ => match f1 in (Fifo n2) return (forall m, S m = n2 -> A) -> A with
+                               | null => fun _ => x
+                               | store _ n3 _ => fun val_pf => val_pf n3 eq_refl
                                end (first' f1)
   end.
 
-Definition first n (f : Fifo (S n)) : A := first' f eq_refl.
-
-(*
-Fixpoint first n (f : Fifo n) : n <> 0 -> A :=
-  match f in Fifo n0 return n0 <> 0 -> A with
-  | emptyFifo => fun pf0 => match pf0 eq_refl with end
-  | enq x _ f1 _ => fun _ => match f1 in (Fifo n2) return (n2 <> 0 -> A) -> A with
-                             | emptyFifo => fun _ => x
-                             | enq _ n3 _ _ => fun val_pf => val_pf (s_n_0 (n := n3))
-                             end (first f1)
-  end.
-*)
-
-(*
-Definition unitFifoPredN n := match n with
-                              | 0 => unit
-                              | S n' => Fifo n'
-                              end.
-
-Fixpoint deq' n (f : Fifo n) : unitFifoPredN n :=
-  match f in Fifo n return unitFifoPredN n with
-  | emptyFifo => tt
-  | enq x n' f' p =>  match n' return unitFifoPredN n' -> (pred n' < size) -> Fifo n' with
-                      | 0 => fun _ _ => emptyFifo
-                      | S _ => fun deq_f p' => enq x deq_f p'
-                      end (deq' f') (predLess p)
-  end.
-
-Definition deq n (f : Fifo (S n)) := deq' f.
-*)
-
-(*
 Fixpoint deq' n (f : Fifo n) : forall m, S m = n -> Fifo (pred n) :=
   match f in Fifo n0 return forall m, S m = n0 -> Fifo (pred n0) with
-  | emptyFifo => fun _ pf0 => match s_n_0 pf0 with end
-  | enq x _ f1 p => fun _ _ => match f1 in (Fifo n2) return (forall m, S m = n2 -> Fifo (pred n2)) -> forall p' : pred n2 < size, Fifo n2 with
-                               | emptyFifo => fun _ _ => emptyFifo
-                               | enq _ n3 _ _ => fun val_pf p'  => enq x (val_pf n3 eq_refl) p'
-                               end (deq' f1) (predLess p)
-  end.
-*)
-
-Fixpoint deq' n (f : Fifo n) : forall m, S m = n -> Fifo (pred n) :=
-  match f in Fifo n0 return forall m, S m = n0 -> Fifo (pred n0) with
-  | emptyFifo => fun _ pf0 => match s_n_0 pf0 with end
-  | enq x _ f1 _ => fun _ _ => match f1 in (Fifo n2) return (forall m, S m = n2 -> Fifo (pred n2)) -> Fifo n2 with
-                               | emptyFifo => fun _ => emptyFifo
-                               | enq _ n3 _ pless => fun val_pf => enq x (val_pf n3 eq_refl) pless
+  | null => fun _ pf0 => match s_n_0 pf0 with end
+  | store x _ f1 => fun _ _ => match f1 in (Fifo n2) return (forall m, S m = n2 -> Fifo (pred n2)) -> Fifo n2 with
+                               | null => fun _ => null
+                               | store _ n3 _ => fun val_pf => store x (val_pf n3 eq_refl)
                                end (deq' f1)
   end.
 
-Definition deq n (f : Fifo (S n)) : Fifo n := deq' f eq_refl.
+Variable size : nat.
 
-(*
-Fixpoint deq n (f : Fifo n) : n <> 0 -> Fifo (pred n) :=
-  match f in Fifo n0 return n0 <> 0 -> Fifo (pred n0) with
-  | emptyFifo => fun pf0 => match pf0 eq_refl with end
-  | enq x _ f1 p => fun _ => match f1 in (Fifo n2) return (n2 <> 0 -> Fifo (pred n2)) -> Fifo n2 with
-                             | emptyFifo => fun _ => emptyFifo
-                             | enq _ n3 _ pless => fun deq_pf => enq x (deq_pf (s_n_0 (n := n3))) pless
-                             end (deq f1)
-  end.
-*)
+Record fifo := mkfifo
+{ num : nat
+; obj : Fifo num
+; bound : num <= size
+}.
 
-Definition isEmpty n (f : Fifo n) : {n = 0} + {n > 0}.
-  refine (match n with
-  | 0 => left _ _
-  | S _ => right _ _
-  end); crush.
-Qed.
-
-(* very trivial lemma *)
-Lemma fifoLessThanSize : forall n, Fifo n -> n <= size.
-  intro; induction 1; intuition.
-Qed.
-
-Definition isFull n (f : Fifo n) : {n = size} + {n < size}.
-  assert ({n = size} + {n <> size}) by (apply eq_nat_dec).
-  assert (n <= size) by (induction f; crush).
+Lemma le_pred_le n m : n <= m -> pred n <= m.
   crush.
 Qed.
 
-(* random lemmas just to fill pages *)
-Lemma enq_first n (f : Fifo (S n)) (notFull : S n < size) (enqVal : A) : first (enq enqVal f notFull) = first f.
-  dep_destruct f; crush.
+Lemma lt_S_le n m : n < m -> S n <= m.
+  crush.
 Qed.
+
+Lemma lt_pred_lt n m : n < m -> pred n < m.
+  crush.
+Qed.
+
+Lemma O_le n : 0 <= n.
+  crush.
+Qed.
+
+Definition emptyFifo :=
+  {| num := 0
+   ; obj := null
+   ; bound := O_le size
+   |}.
+
+Definition enq x (f : fifo) (pf : num f < size) : fifo :=
+  {| num := S (num f)
+   ; obj := store x (obj f)
+   ; bound := lt_S_le pf
+   |}.
+
+Definition first (f : fifo) : forall m, S m = num f -> A := first' (obj f).
+
+Definition deq (f : fifo) m (pf : S m = num f) : fifo :=
+  {| num := pred (num f)
+   ; obj := deq' (obj f) pf
+   ; bound :=  le_pred_le (bound f)
+   |}.
 
 (* a step in a fifo, which contains a source and a sink
      a) enq: only enqueue from source happens (source changes from Some to None)
@@ -149,9 +87,10 @@ Qed.
           State of the FIFO must be maintained correctly
      d) nothing : nothing happens, simulates other activities happening in the network
  *)
-Inductive fifoStep : forall n, Fifo n -> option A -> option A -> forall n', Fifo n' -> option A -> option A -> Prop :=
-| Enq : forall n (f : Fifo n) (notFull : n < size) (enqVal : A) (deqVal : option A), fifoStep f (Some enqVal) deqVal (enq enqVal f notFull) None deqVal
-| Deq : forall n (f : Fifo (S n)) (enqVal : option A), fifoStep f enqVal None (deq f) enqVal (Some (first f))
-| EnqDeq : forall n (f : Fifo (S n)) (notFull : S n < size) (enqVal : A), fifoStep f (Some enqVal) None (deq (enq enqVal f notFull)) None (Some (first f))
-| NoFifoAction : forall n (f : Fifo n) (enqVal deqVal : option A), fifoStep f enqVal deqVal f enqVal deqVal.
+Inductive fifoStep : fifo -> option A -> option A -> fifo -> option A -> option A -> Prop :=
+| Enq : forall enqVal f (notFull : num f < size) deqVal, fifoStep f (Some enqVal) deqVal (enq enqVal f notFull) None deqVal
+| Deq : forall f m (notEmpty: S m = num f) enqVal, fifoStep f enqVal None (deq f notEmpty) enqVal (Some (first f notEmpty))
+| EnqDeq : forall f (notFull : num f < size) m (notEmpty: S m = num f) enqVal, fifoStep f (Some enqVal) None (enq enqVal (deq f notEmpty) (lt_pred_lt notFull)) None (Some (first f notEmpty))
+| NoFifoAction : forall f enqVal deqVal, fifoStep f enqVal deqVal f enqVal deqVal.
+
 End Fifo.
